PdlParallelStoring/Completeness.lean
@@ -1,0 +1,36 @@
+import Mathlib.Logic.Basic
+import Mathlib.Data.Set.Insert
+
+import PdlParallelStoring.AxiomaticSystem
+import PdlParallelStoring.Properties
+
+def IsConsistent (s : Set Φ) : Prop :=
+  ¬ ∃ (φs : List Φ), (∀ φ ∈ φs, φ ∈ s) ∧ (⊢ ((φs.foldr (· ∧ ·) ⊤') → ⊥'))
+
+def IsMaximal (s : Set Φ) : Prop :=
+  IsConsistent s ∧ ∀ {φ : Φ}, (φ ∉ s) → ¬ IsConsistent (s ∪ {φ})
+
+def MaximalConsistentSet : Type :=
+  {s : Set Φ // IsMaximal s}
+
+def CanonicalFrame : Frame where
+  W := MaximalConsistentSet
+  R := sorry
+  nonempty := sorry
+
+def CanonicalModel : Model where
+  F := CanonicalFrame
+  V := sorry
+
+instance canonical_proper : Proper CanonicalFrame := by
+  sorry
+
+instance canonical_standard : Standard CanonicalModel := by
+  sorry
+
+instance : ProperStandard CanonicalModel where
+  toStandard := canonical_standard
+  toProper := canonical_proper
+
+theorem completeness : ∀ {φ : Φ}, (¬ ⊢ φ) → ∃ (M : Model) (_ : ProperStandard M), ¬ (M ⊨ φ) := by
+  sorry
